theories/ValueOpts/ConstantPropagation.v
@@ -3,7 +3,7 @@ Require Import CSet Le Coq.Classes.RelationClasses.
 Require Import Plus Util AllInRel Map Indexwise.
 Require Import CSet Val Var Env IL Sim Fresh Annotation LabelsDefined DecSolve OptionR.
 
-Require Import RenamedApart SetOperations Eqn ValueOpts Infra.Lattice WithTop.
+Require Import RenamedApart SetOperations Eqn Infra.Lattice WithTop.
 
 Set Implicit Arguments.
 Unset Printing Records.
@@ -93,41 +93,31 @@ Qed.
 
 Inductive cp_sound (AE:onv (withTop val)) :
                      list (params*list aval)
-                     -> list bool
                      -> stmt
                      -> ann bool
                      -> Prop :=
-| CPOpr (x:var) Cp Rch (b:bool) r e s
-  : cp_sound AE Cp Rch s r
+| CPOpr (x:var) Cp (b:bool) r e s
+  : cp_sound AE Cp s r
     -> (b -> exp_eval AE e = AE x)
-    -> (b -> getAnn r)
-    -> cp_sound AE Cp Rch (stmtLet x e s) (ann1 b r)
-| CPIf Cp Rch e (b:bool) s1 s2 (r1 r2:ann bool)
-       (Cond1:cp_sound AE Cp Rch s1 r1)
-       (Cond2:cp_sound AE Cp Rch s2 r2)
-       (Reach1:b -> op_eval AE e <> None -> aval2bool (op_eval AE e) <> Some (wTA false) -> getAnn r1)
-       (Reach2:b -> poLe (Some (wTA val_false)) (op_eval AE e) -> getAnn r2)
-  : cp_sound AE Cp Rch (stmtIf e s1 s2) (ann2 b r1 r2)
-| CPGoto l Y Cp Rch Z aY (b bf:bool)
+    -> cp_sound AE Cp (stmtLet x e s) (ann1 b r)
+| CPIf Cp e (b:bool) s1 s2 (r1 r2:ann bool)
+       (Cond1:cp_sound AE Cp s1 r1)
+       (Cond2:cp_sound AE Cp s2 r2)
+  : cp_sound AE Cp (stmtIf e s1 s2) (ann2 b r1 r2)
+| CPGoto l Y Cp Z aY (b bf:bool)
   : get Cp (counted l) (Z,aY)
-    -> get Rch (counted l) bf
     -> length Z = length Y
     -> (b -> PIR2 poLe (List.map (op_eval AE) Y) aY)
-    -> (b -> bf)
-    -> cp_sound AE Cp Rch (stmtApp l Y) (ann0 b)
-| CPReturn Cp Rch e b
-  : cp_sound AE Cp Rch (stmtReturn e) (ann0 b)
-| CPLet Cp Rch F t (b:bool) (rF:list (ann bool)) (r:ann bool) (rfLen:❬F❭=❬rF❭)
-   (Reach1:b -> getAnn r)
+    -> cp_sound AE Cp (stmtApp l Y) (ann0 b)
+| CPReturn Cp e b
+  : cp_sound AE Cp (stmtReturn e) (ann0 b)
+| CPLet Cp F t (b:bool) (rF:list (ann bool)) (r:ann bool) (rfLen:❬F❭=❬rF❭)
   : (forall n Zs r,
         get F n Zs ->
         get rF n r ->
-        cp_sound AE (List.map (fun Zs => (fst Zs, lookup_list AE (fst Zs))) F ++ Cp)
-                 (getAnn ⊝ rF ++ Rch)
-                 (snd Zs) r)
-    -> cp_sound AE (List.map (fun Zs => (fst Zs, lookup_list AE (fst Zs))) F ++ Cp)
-               (getAnn ⊝ rF ++ Rch) t r
-    -> cp_sound AE Cp Rch (stmtFun F t) (annF b rF r).
+        cp_sound AE (List.map (fun Zs => (fst Zs, lookup_list AE (fst Zs))) F ++ Cp) (snd Zs) r)
+    -> cp_sound AE (List.map (fun Zs => (fst Zs, lookup_list AE (fst Zs))) F ++ Cp) t r
+    -> cp_sound AE Cp (stmtFun F t) (annF b rF r).
 
 Definition indexwise_R1 {A} (P:A->Prop) LA :=
 forall n a, get LA n a -> P a.
@@ -144,62 +134,26 @@ intros. destruct (Rdec 0 a).
 - right; intro HH. eapply n; hnf; intros; eapply HH; eauto using get.
 Defined.
 
-Instance cp_sound_dec AE Rch ZL s r : Computable (cp_sound AE ZL Rch s r).
+Instance cp_sound_dec AE ZL s r : Computable (cp_sound AE ZL s r).
 Proof.
-  hnf. revert AE Rch ZL r; sind s; intros; destruct s; destruct r; try dec_solve.
+  hnf. revert AE ZL r; sind s; intros; destruct s; destruct r; try dec_solve.
   - edestruct (IH s); eauto;
       decide (a -> exp_eval AE e = AE x); try dec_solve;
-        decide (a -> getAnn r); try dec_solve.
-  - edestruct (IH s2 ltac:(eauto) AE Rch ZL); eauto; [| dec_solve];
-      edestruct (IH s1 ltac:(eauto) AE Rch ZL); eauto; [| dec_solve];
+        try dec_solve.
+  - edestruct (IH s2 ltac:(eauto) AE ZL); eauto; [| dec_solve];
+      edestruct (IH s1 ltac:(eauto) AE ZL); eauto; [| dec_solve];
         decide (op_eval AE e = None);
         decide (aval2bool (op_eval AE e) = Some (wTA false));
         (decide (poLe (Some (wTA val_false)) (op_eval AE e)));
         decide (a); decide (getAnn r1); decide (getAnn r2); try dec_solve.
   - destruct (get_dec ZL (counted l)) as [[[]]|]; try dec_solve.
-    destruct (get_dec Rch (counted l)) as [[]|]; try dec_solve.
     decide (length l0 = length Y); try dec_solve.
     decide (a -> PIR2 poLe (List.map (op_eval AE) Y) l1);
       try dec_solve.
-    decide (a -> x); try dec_solve.
   - assert (SZ:size s < size (stmtFun F s)) by eauto.
     decide (❬F❭=❬sa❭); [|dec_solve].
-    edestruct (IH s SZ AE (getAnn ⊝ sa ++ Rch) (List.map (fun Zs => (fst Zs, lookup_list AE (fst Zs))) F ++ ZL) r); [|dec_solve].
+    edestruct (IH s SZ AE (List.map (fun Zs => (fst Zs, lookup_list AE (fst Zs))) F ++ ZL) r); [|dec_solve].
     exploit (@indexwise_R2_dec _ _ (fun Zs r => cp_sound AE ((fun Zs0 : params * stmt => (fst Zs0,
-        lookup_list AE (fst Zs0))) ⊝ F ++ ZL)(getAnn ⊝ sa ++ Rch)  (snd Zs) r) F); eauto.
-    intros. eapply IH; eauto. destruct H;[|dec_solve].
-    decide (a -> getAnn r); dec_solve.
+        lookup_list AE (fst Zs0))) ⊝ F ++ ZL) (snd Zs) r) F); eauto.
+    intros. eapply IH; eauto. destruct H; dec_solve.
 Defined.
-
-Require Import Reachability.
-
-Definition cop2bool AE e := aval2bool (op_eval AE e).
-
-Lemma impb_lift (b b':bool)
-  : (b -> b')
-    -> impb b b'.
-Proof.
-  unfold impb; cases; eauto.
-Qed.
-
-Local Hint Resolve impb_lift.
-
-Lemma test AE ZL Rch s r
-  : cp_sound AE ZL Rch s r
-    -> reachability (cop2bool AE) Sound Rch s r.
-Proof.
-  intros CPS.
-  general induction CPS; econstructor; simpl; eauto.
-  - intros. unfold cop2bool in *. eapply Reach1; eauto.
-    intro. rewrite H2 in *. simpl in *. congruence.
-  - intros. unfold cop2bool in *. eapply Reach2; eauto.
-    case_eq (op_eval AE e); intros. rewrite H2 in *. simpl in *.
-    simpl in *; destruct w; try congruence; eauto.
-    econstructor; eauto. econstructor; eauto.
-    simpl in *.
-    case_eq (val2bool a); intros; rewrite H3 in *; try congruence.
-    unfold val2bool in H3. cases in H3.
-    econstructor; eauto. econstructor; eauto. reflexivity.
-    congruence.
-    rewrite H2 in H. simpl in *. congruence.
-Qed.
