theories/UCE.v
@@ -268,8 +268,21 @@ Proof.
     pone_step. left. eauto.
 Qed.
 
+Lemma poLe_impl_use (a b:bool)
+  : poLe a b
+    -> a
+    -> b.
+Proof.
+  destruct a, b; firstorder.
+Qed.
+
+Opaque poLe.
+
+Local Hint Resolve poLe_impl_use.
+
+
 Lemma sim_I RL r L L' V s (a:ann bool) (Ann:getAnn a)
- (RCH: reachability op2bool Sound RL s a)
+ (RCH: reachability cop2bool Sound RL s a)
  (LSIM:labenv_sim Bisim (sim r) SR RL L L')
   : sim r Bisim (L,V, s) (L',V, compile RL s a).
 Proof.
@@ -278,7 +291,7 @@ Proof.
   - destruct e.
     + eapply (sim_let_op il_statetype_I); eauto.
     + eapply (sim_let_call il_statetype_I); eauto.
-  - eapply (sim_if_elim il_statetype_I); intros; eauto.
+  - eapply (sim_if_elim il_statetype_I); intros; eauto 20 using op2bool_cop2bool_not_some.
   - assert (b=true). destruct a0, b; isabsurd; eauto. subst.
     eapply labenv_sim_app; eauto.
     + hnf; simpl. split; eauto using zip_get.
@@ -297,7 +310,7 @@ Proof.
 Qed.
 
 Lemma sim_UCE V s a
-  : reachability op2bool Sound nil s a
+  : reachability cop2bool Sound nil s a
     -> getAnn a
     -> @sim I.state _ I.state _ bot3 Bisim (nil,V, s) (nil,V, compile nil s a).
 Proof.
@@ -385,7 +398,7 @@ Proof.
 Qed.
 
 Lemma sim_F RL r L L' V s (a:ann bool) (Ann:getAnn a)
- (UC: reachability op2bool Sound RL s a)
+ (UC: reachability cop2bool Sound RL s a)
  (LSIM:labenv_sim Bisim (sim r) SR RL L L')
   : sim r Bisim (L,V, s) (L',V, compile RL s a).
 Proof.
@@ -394,7 +407,7 @@ Proof.
   - destruct e.
     + eapply (sim_let_op il_statetype_F); eauto.
     + eapply (sim_let_call il_statetype_F); eauto.
-  - eapply (sim_if_elim il_statetype_F); intros; eauto.
+  - eapply (sim_if_elim il_statetype_F); intros; eauto 20 using op2bool_cop2bool_not_some.
   - assert (b=true). destruct a0, b; isabsurd; eauto. subst.
     eapply labenv_sim_app; eauto.
     + hnf; simpl. split; eauto using zip_get.
@@ -413,7 +426,7 @@ Proof.
 Qed.
 
 Lemma sim_UCE V s a
-  : reachability op2bool Sound nil s a
+  : reachability cop2bool Sound nil s a
     -> getAnn a
     -> @sim F.state _ F.state _ bot3 Bisim (nil,V, s) (nil,V, compile nil s a).
 Proof.
@@ -426,15 +439,26 @@ End F.
 
 (** ** UCE respects parameter/argument matching *)
 
+
+Opaque poLe.
+
 Lemma UCE_paramsMatch PL RL s lv
-  : reachability op2bool Sound RL s lv
+  : reachability cop2bool Sound RL s lv
     -> getAnn lv
     -> paramsMatch s PL
     -> paramsMatch (compile RL s lv) (filter_by (fun b => b) RL PL).
 Proof.
   intros UC Ann PM.
   general induction UC; inv PM; simpl in * |- *; repeat cases; eauto using paramsMatch.
-  - specialize (H NOTCOND0). specialize (H0 NOTCOND). subst. simpl in *.
+  - rewrite op2bool_cop2bool in COND.
+    eapply IHUC1; eauto. exploit H; eauto.
+    rewrite COND. intro. clear_trivial_eqs.
+  - rewrite op2bool_cop2bool in COND.
+    eapply IHUC2; eauto. exploit H0; eauto.
+    rewrite COND. intro. clear_trivial_eqs.
+  - eapply op2bool_cop2bool_not_some in NOTCOND.
+    eapply op2bool_cop2bool_not_some in NOTCOND0.
+    exploit H; eauto. exploit H0; eauto.
     econstructor; eauto.
   - simpl in *.
     exploit (get_filter_by (fun b => b) H H3). destruct a,b; isabsurd; eauto.
@@ -486,7 +510,7 @@ Fixpoint compile_live (s:stmt) (a:ann (set var)) (b:ann bool) : ann (set var) :=
 
 Lemma compile_live_incl i uci ZL LV RL s lv uc
   : true_live_sound i ZL LV s lv
-    -> reachability op2bool uci RL s uc
+    -> reachability cop2bool uci RL s uc
     -> getAnn (compile_live s lv uc) ⊆ getAnn lv.
 Proof.
   intros LS UC.
@@ -500,7 +524,7 @@ Proof.
 Qed.
 
 Lemma UCE_live i ZL LV RL s uc lv
-  : reachability op2bool Sound RL s uc
+  : reachability cop2bool Sound RL s uc
     -> getAnn uc
     -> true_live_sound i ZL LV s lv
     -> true_live_sound i (filter_by (fun b => b) RL ZL)
@@ -513,9 +537,19 @@ Proof.
   - econstructor; eauto using compile_live_incl with cset.
     intros. eapply H. destruct H1; eauto.
     left. eapply compile_live_incl; eauto.
-  - repeat cases; eauto. econstructor; eauto; intros.
-    + rewrite compile_live_incl; eauto.
-    + rewrite compile_live_incl; eauto.
+  - repeat cases; eauto.
+    + eapply H0; eauto.
+      exploit H9; eauto.
+      rewrite op2bool_cop2bool in COND; eauto.
+      rewrite COND. intro. clear_trivial_eqs.
+    + eapply op2bool_cop2bool_not_some in NOTCOND.
+      eapply H2; eauto.
+      exploit H10; eauto.
+    + exploit H9; eauto using op2bool_cop2bool_not_some.
+      exploit H10; eauto using op2bool_cop2bool_not_some.
+      econstructor; intros; eauto; try congruence.
+      rewrite compile_live_incl; eauto.
+      rewrite compile_live_incl; eauto.
   - repeat get_functional. simpl in *.
     assert (❬take (labN l) RL❭ = ❬take (labN l) ZL❭).
     eapply get_range in H. eapply get_range in H7.
@@ -577,7 +611,7 @@ Qed.
 
 Lemma trueIsCalled_compileF_not_nil
       (s : stmt) (slv : ann bool) k F als RL x
-  : reachability op2bool Sound (getAnn ⊝ als ++ RL) s slv
+  : reachability cop2bool Sound (getAnn ⊝ als ++ RL) s slv
     -> getAnn slv
     -> isCalled true s (LabI k)
     -> get als k x
@@ -602,17 +636,17 @@ Lemma UCE_callChain RL F als t alt l' k ZsEnd aEnd n
       (IH : forall k Zs,
           get F k Zs ->
        forall (RL : 〔bool〕) (lv : ann bool) (n : nat),
-       reachability op2bool SoundAndComplete RL (snd Zs) lv ->
+       reachability cop2bool SoundAndComplete RL (snd Zs) lv ->
        (isCalled true) (snd Zs) (LabI n) ->
        getAnn lv ->
        (isCalled true) (compile RL (snd Zs) lv)
                 (LabI (countTrue (take n RL))))
-  (UC:reachability op2bool SoundAndComplete (getAnn ⊝ als ++ RL) t alt)
+  (UC:reachability cop2bool SoundAndComplete (getAnn ⊝ als ++ RL) t alt)
   (LEN: ❬F❭ = ❬als❭)
   (UCF:forall (n : nat) (Zs : params * stmt) (a : ann bool),
        get F n Zs ->
        get als n a ->
-       reachability op2bool SoundAndComplete (getAnn ⊝ als ++ RL) (snd Zs) a)
+       reachability cop2bool SoundAndComplete (getAnn ⊝ als ++ RL) (snd Zs) a)
   (Ann: getAnn alt)
   (IC: isCalled true t (LabI l'))
   (CC: callChain (isCalled true) F (LabI l') (LabI k))
@@ -654,7 +688,7 @@ Lemma UCE_callChain' RL F als l' k
       (IH : forall k Zs,
           get F k Zs ->
        forall (RL : 〔bool〕) (lv : ann bool) (n : nat),
-       reachability op2bool SoundAndComplete RL (snd Zs) lv ->
+       reachability cop2bool SoundAndComplete RL (snd Zs) lv ->
        (isCalled true) (snd Zs) (LabI n) ->
        getAnn lv ->
        (isCalled true) (compile RL (snd Zs) lv)
@@ -663,7 +697,7 @@ Lemma UCE_callChain' RL F als l' k
   (UCF:forall (n : nat) (Zs : params * stmt) (a : ann bool),
        get F n Zs ->
        get als n a ->
-       reachability op2bool SoundAndComplete (getAnn ⊝ als ++ RL) (snd Zs) a)
+       reachability cop2bool SoundAndComplete (getAnn ⊝ als ++ RL) (snd Zs) a)
   (Ann: get (getAnn ⊝ als ++ RL) l' true)
   (CC: callChain (isCalled true) F (LabI l') (LabI k))
 : callChain (isCalled true)
@@ -685,7 +719,7 @@ Proof.
 Qed.
 
 Lemma UCE_trueIsCalled RL s lv n
-  : reachability op2bool SoundAndComplete RL s lv
+  : reachability cop2bool SoundAndComplete RL s lv
     -> isCalled true s (LabI n)
     -> getAnn lv
     -> isCalled true (compile RL s lv) (LabI (countTrue (take n RL))).
@@ -695,7 +729,15 @@ Proof.
   sind s; simpl; intros; invt reachability; invt isCalled;
     simpl in *; eauto using isCalled.
   - repeat cases; eauto using isCalled.
+    + eapply IH; eauto.
+      rewrite <- H0; eauto using op2bool_cop2bool_not_some.
+    + econstructor; eauto. eapply IH; eauto.
+      rewrite <- H0; eauto using op2bool_cop2bool_not_some.
   - repeat cases; eauto using isCalled.
+    + eapply IH; eauto.
+      rewrite <- H1; eauto using op2bool_cop2bool_not_some.
+    + econstructor 3; eauto. eapply IH ; eauto.
+      rewrite <- H1; eauto using op2bool_cop2bool_not_some.
   - eapply callChain_cases in H8. destruct H8; subst.
     + cases.
       * exploit (IH t) as IHt; eauto.
@@ -729,8 +771,8 @@ Lemma UCE_isCalledFrom RL F als t alt n (Len:❬F❭ = ❬als❭)
   : (forall (n : nat) (Zs : params * stmt) (a : ann bool),
        get F n Zs ->
        get als n a ->
-       reachability op2bool SoundAndComplete (getAnn ⊝ als ++ RL) (snd Zs) a)
-    -> reachability op2bool SoundAndComplete (getAnn ⊝ als ++ RL) t alt
+       reachability cop2bool SoundAndComplete (getAnn ⊝ als ++ RL) (snd Zs) a)
+    -> reachability cop2bool SoundAndComplete (getAnn ⊝ als ++ RL) t alt
     -> getAnn alt
     -> isCalledFrom (isCalled true) F t (LabI n)
     -> n < ❬F❭
@@ -751,13 +793,17 @@ Proof.
 Qed.
 
 Lemma UCE_noUnreachableCode RL s lv
-  : reachability op2bool SoundAndComplete RL s lv
+  : reachability cop2bool SoundAndComplete RL s lv
     -> getAnn lv
     -> noUnreachableCode (isCalled true) (compile RL s lv).
 Proof.
   intros Live GetAnn.
   induction Live; simpl in *; repeat cases; eauto using noUnreachableCode.
-  - specialize (H NOTCOND0). specialize (H0 NOTCOND). subst.
+  - rewrite op2bool_cop2bool in COND. rewrite H in GetAnn; eauto.
+    rewrite COND; eauto. intro. clear_trivial_eqs.
+  - eapply op2bool_cop2bool_not_some in NOTCOND. rewrite H0 in GetAnn; eauto.
+  - exploit H; eauto using op2bool_cop2bool_not_some.
+    exploit H0; eauto using op2bool_cop2bool_not_some. subst.
     simpl in *. econstructor; eauto.
   - rewrite Heq; clear Heq.
     econstructor; eauto using noUnreachableCode.
@@ -818,7 +864,7 @@ Fixpoint compile_renamedApart (s:stmt) (a:ann (set var * set var)) (b:ann bool)
 
 Lemma compile_renamedApart_pes RL s an al
   : renamedApart s an
-    -> reachability op2bool Sound RL s al
+    -> reachability cop2bool Sound RL s al
     -> prod_eq Equal Subset (getAnn (compile_renamedApart s an al)) (getAnn an).
 Proof.
   intros RA RCH.
@@ -847,7 +893,7 @@ Qed.
 
 Lemma UCE_renamedApart RL s lv G
   : renamedApart s G
-    -> reachability op2bool Sound RL s lv
+    -> reachability cop2bool Sound RL s lv
     -> renamedApart (compile RL s lv) (compile_renamedApart s G lv).
 Proof.
   intros RA RCH.
@@ -918,7 +964,7 @@ Require Import VarP.
 
 Lemma UCE_var_P (P:nat -> Prop) RL (s:stmt) a
       (VP:var_P P s)
-      (RCH: reachability op2bool Sound RL s a)
+      (RCH: reachability cop2bool Sound RL s a)
   : var_P P (compile RL s a).
 Proof.
   general induction VP; invt reachability; simpl;
